ifc/abstract.v
@@ -1,7 +1,7 @@
 From mathcomp Require Import
   ssreflect ssrfun ssrbool ssrnat eqtype seq choice fintype finfun.
 From CoqUtils Require Import hseq ord partmap word.
-From MicroPolicies Require Import lib.utils common.types ifc.labels.
+From MicroPolicies Require Import lib.utils common.types ifc.labels ifc.common.
 
 Set Implicit Arguments.
 Unset Strict Implicit.
@@ -21,9 +21,10 @@ Local Notation word := (mword mt).
 Local Notation atom := (atom word L).
 
 Record state := State {
-  mem     : {partmap mword mt -> instr mt + atom};
-  regs    : {partmap reg mt -> atom};
-  pc      : atom
+  mem        : {partmap mword mt -> instr mt + atom};
+  regs       : {partmap reg mt -> atom};
+  pc         : atom;
+  call_stack : seq (call_frame mt L)
 }.
 
 Local Open Scope word_scope.
@@ -32,29 +33,29 @@ Local Open Scope label_scope.
 Implicit Type s : state.
 
 Definition step s : option (state * option atom):=
-  let: State mem regs pc@lpc := s in
+  let: State mem regs pc@lpc stk := s in
   if mem pc is Some i then
     if i is inl i then
       match i with
-      | Nop => Some (State mem regs (pc + 1)@lpc, None)
+      | Nop => Some (State mem regs (pc + 1)@lpc stk, None)
       | Const k r =>
         do! regs <- updm regs r (swcast k)@⊥;
-        Some (State mem regs (pc + 1)@lpc, None)
+        Some (State mem regs (pc + 1)@lpc stk, None)
       | Mov r1 r2 =>
         do! v <- regs r1;
         do! regs <- updm regs r2 v;
-        Some (State mem regs (pc + 1)@lpc, None)
+        Some (State mem regs (pc + 1)@lpc stk, None)
       | Binop o r1 r2 r3 =>
         do! v1 <- regs r1;
         do! v2 <- regs r2;
         do! regs <- updm regs r3 (binop_denote o (vala v1) (vala v2))@(taga v1 ⊔ taga v2);
-        Some (State mem regs (pc + 1)@lpc, None)
+        Some (State mem regs (pc + 1)@lpc stk, None)
       | Load r1 r2 =>
         do! v1 <- regs r1;
         do! v2 <- mem (vala v1);
         if v2 is inr v2 then
           do! regs <- updm regs r2 (vala v2)@(taga v1 ⊔ taga v2);
-          Some (State mem regs (pc + 1)@lpc, None)
+          Some (State mem regs (pc + 1)@lpc stk, None)
         else None
       | Store r1 r2 =>
         do! v1 <- regs r1;
@@ -64,21 +65,21 @@ Definition step s : option (state * option atom):=
           if taga v1 ⊔ lpc ⊑ taga vold then
             do! mem <- updm mem (vala v1)
                                 (inr (vala v2)@(taga v1 ⊔ taga v2 ⊔ lpc));
-            Some (State mem regs (pc + 1)@lpc, None)
+            Some (State mem regs (pc + 1)@lpc stk, None)
           else None
         else None
       | Jump r =>
         do! v <- regs r;
-        Some (State mem regs (vala v)@(taga v ⊔ lpc), None)
+        Some (State mem regs (vala v)@(taga v ⊔ lpc) stk, None)
       | Bnz r x =>
         do! v <- regs r;
         let pc' := pc + if vala v == 0 then 1
                         else swcast x in
-        Some (State mem regs pc'@(taga v ⊔ lpc), None)
+        Some (State mem regs pc'@(taga v ⊔ lpc) stk, None)
       | Jal r =>
         do! v <- regs r;
         do! regs <- updm regs ra (pc + 1)@(taga v ⊔ lpc);
-        Some (State mem regs (vala v)@(taga v ⊔ lpc), None)
+        Some (State mem regs (vala v)@(taga v ⊔ lpc) stk, None)
       | JumpEpc => None
       | AddRule => None
       | GetTag _ _ => None
@@ -91,7 +92,7 @@ Definition step s : option (state * option atom):=
     do! out   <- regs r_arg;
     let r_pc  := taga raddr in
     let r_out := taga out in
-    Some (State mem regs raddr,
+    Some (State mem regs raddr stk,
           Some (vala out)@(r_pc ⊔ r_out))
   else None.
 
