ifc/common.v
@@ -1,0 +1,34 @@
+From mathcomp Require Import ssreflect ssrfun ssrbool ssrnat eqtype seq.
+From CoqUtils Require Import hseq ord partmap word.
+From MicroPolicies Require Import lib.utils common.types ifc.labels.
+
+Set Implicit Arguments.
+Unset Strict Implicit.
+Unset Printing Implicit Defensive.
+
+Section CallFrame.
+
+Variable mt : machine_types.
+Variable L : labType.
+
+Record call_frame := CallFrame {
+  cf_pc   : atom (mword mt) L;
+  cf_lab  : L;
+  cf_regs : {partmap reg mt -> atom (mword mt) L}
+}.
+
+Definition tuple_of_call_frame cf :=
+  (cf_pc cf, cf_lab cf, cf_regs cf).
+
+Definition call_frame_of_tuple cf :=
+  let: (pc, lab, regs) := cf in
+  CallFrame pc lab regs.
+
+Lemma tuple_of_call_frameK : cancel tuple_of_call_frame call_frame_of_tuple.
+Proof. by case. Qed.
+
+Definition call_frame_eqMixin := CanEqMixin tuple_of_call_frameK.
+Canonical call_frame_eqType :=
+  Eval hnf in EqType call_frame call_frame_eqMixin.
+
+End CallFrame.
